Make progress on backendProof
Change installed_def so that it says the bitmaps are installed in
memory (not just that there is space for them).

The end of the proof has some innocuous looking conditions left to
prove, that seem like they should have been handled earlier.

compiler/backend/proofs/backendProofScript.sml
@@ -177,6 +177,19 @@ val DISJOINT_INTER = Q.store_thm("DISJOINT_INTER",
   `DISJOINT b c ⇒ DISJOINT (a ∩ b) (a ∩ c)`,
   rw[IN_DISJOINT] \\ metis_tac[]);
 
+val args = full_make_init_semantics_fail |> concl |> dest_imp |> #1 |> dest_conj |> #1 |> rand
+val defn = full_make_init_semantics_fail |> concl |> dest_imp |> #1 |> dest_conj |> #2 |> lhs
+val full_init_pre_fail_def =
+  Define`full_init_pre_fail ^args = ^defn`;
+
+val full_make_init_bitmaps = Q.prove(
+  `full_init_pre_fail args = SOME x ==>
+    (full_make_init args).bitmaps = FST args`,
+  PairCases_on`args` \\
+  fs [full_make_init_def,stack_allocProofTheory.make_init_def,
+      stack_removeProofTheory.make_init_any_bitmaps]
+  \\ every_case_tac \\ fs [] \\ fs [full_init_pre_fail_def]);
+
 (* -- *)
 
 (* TODO: Move somewhere, not sure where though *)
@@ -440,13 +453,13 @@ val word_in_byte_mem_def = Define`
 *)
 val installed_def = Define`
   installed bytes bitmaps ffi_names ffi (r1,r2) mc_conf ms ⇔
-    ∃t m io_regs bitmap_ptr.
+    ∃t m io_regs bitmap_ptr bitmaps_dm.
+      (*let bitmaps_dm = { w | bitmap_ptr <=+ w ∧ w <+ bitmap_ptr + bytes_in_word * n2w (LENGTH bitmaps)} in*)
       let heap_stack_dm = { w | t.regs r1 <=+ w ∧ w <+ t.regs r2 } in
-      let bitmaps_dm = { w | bitmap_ptr <=+ w ∧ w <+ bitmap_ptr + n2w (LENGTH bitmaps)} in
       good_init_state mc_conf ms ffi bytes t m (heap_stack_dm ∪ bitmaps_dm) io_regs ∧
       DISJOINT heap_stack_dm bitmaps_dm ∧
       m (t.regs r1) = Word bitmap_ptr ∧
-      (* TODO: need an additional assumption on where the bitmaps are *)
+      word_list bitmap_ptr (MAP Word bitmaps) (fun2set (m,byte_aligned ∩ bitmaps_dm)) ∧
       ffi_names = SOME mc_conf.ffi_names`;
 
 val byte_aligned_MOD = Q.store_thm("byte_aligned_MOD",`
@@ -950,8 +963,10 @@ val compile_correct = Q.store_thm("compile_correct",
         match_mp_tac fun2set_disjoint_union \\
         conj_tac >- (
           match_mp_tac DISJOINT_INTER
-          \\ simp[DISJOINT_SYM] ) \\
-        reverse conj_tac >- (
+          \\ metis_tac[DISJOINT_SYM] ) \\
+        conj_tac >- (
+          fs[attach_bitmaps_def] )
+        \\ (
           match_mp_tac word_list_exists_imp>>
           fs [addresses_thm]>>
           fs[mc_conf_ok_def]>>
@@ -985,8 +1000,7 @@ val compile_correct = Q.store_thm("compile_correct",
           \\ Cases_on `a` \\ Cases_on `b`
           \\ full_simp_tac std_ss [WORD_LS,addressTheory.word_arith_lemma2]
           \\ fs [] \\ match_mp_tac DIV_LESS_DIV \\ fs []
-          \\ rfs [] \\ fs [] \\ match_mp_tac MOD_SUB_LEMMA \\ fs [])>>
-        cheat (* if the first is aligned, the rest should be - word_list lemma? *) )
+          \\ rfs [] \\ fs [] \\ match_mp_tac MOD_SUB_LEMMA \\ fs []) \\
     CONJ_TAC>- (
       simp[EVERY_MEM,MEM_MAP,PULL_EXISTS,FORALL_PROD,Abbr`c4`]>>
       rw[]>-
@@ -1052,9 +1066,9 @@ val compile_correct = Q.store_thm("compile_correct",
       asm_exists_tac>>
       simp[]>>Cases>> simp[]))>>
   strip_tac \\
-
   Cases_on`full_init_pre_fail stack_args` >- (
     qunabbrev_tac`stack_args` \\
+    fs[full_init_pre_fail_def] \\
     drule full_make_init_semantics_fail \\
     strip_tac \\ rfs[] \\
     match_mp_tac (GEN_ALL (MP_CANON implements_trans)) \\
@@ -1064,29 +1078,6 @@ val compile_correct = Q.store_thm("compile_correct",
     simp[Once CONJ_COMM] \\
     asm_exists_tac \\ simp[] \\
     metis_tac[dataPropsTheory.Resource_limit_hit_implements_semantics] ) \\
-  `full_init_pre stack_args` by (
-    fs[full_init_pre_def,full_init_shared_def,Abbr`stack_args`] \\
-    IF_CASES_TAC \\ fs[] >- (
-      fs[IS_SOME_EXISTS]>>
-      drule make_init_opt_imp_bitmaps_limit>>simp[]>>
-      ntac 4 strip_tac>>
-      imp_res_tac ALOOKUP_MEM>>
-      `MEM k (MAP FST p6) ∧ MEM prog' (MAP SND p6)` by
-        metis_tac[MEM_MAP,FST,SND]>>
-      qpat_x_assum`MAP FST p6 = _` SUBST_ALL_TAC>>
-      fs[EVERY_MEM]
-      >-
-        (qpat_x_assum`MEM k _` mp_tac>>
-        EVAL_TAC>>
-        rpt(pop_assum kall_tac)>>
-        DECIDE_TAC)
-      >>
-        first_x_assum drule>>
-        EVAL_TAC>>
-        fs[])>>
-    qhdtm_x_assum`(~)`mp_tac \\
-    simp[full_init_pre_fail_def] ) \\
-
   fs[Abbr`word_st`] \\ rfs[] \\
   match_mp_tac (GEN_ALL (MP_CANON implements_trans)) \\
   qmatch_assum_abbrev_tac`z InitGlobals_location ∈ _ {_}` \\
@@ -1137,6 +1128,8 @@ val compile_correct = Q.store_thm("compile_correct",
   asm_exists_tac \\ simp[] \\
   simp[Abbr`stack_args`] \\
   match_mp_tac stack_to_labProofTheory.full_make_init_semantics \\
+  qhdtm_x_assum`full_init_pre_fail`mp_tac \\
+  simp[full_init_pre_fail_def] \\ strip_tac \\
   simp[]);
 
 val _ = export_theory();
